code/experimental/curve25519/vale_25519.h
@@ -7,11 +7,52 @@ extern uint64_t sub1(const uint64_t* dst, const uint64_t* in_a, uint64_t b);
 extern uint64_t sub(const uint64_t* dst, const uint64_t* in_a, const uint64_t* in_b);
 
 static inline
-uint64_t mul1_add(const uint64_t* dst, const uint64_t* in_a, uint64_t b) {
+uint64_t mul1_add(const uint64_t* dst, const uint64_t* in_a, uint64_t x, const uint64_t* in_b) {
   uint64_t tmp[4] = {0};
-  uint64_t s5 = mul1(tmp,in_a,b);
-  uint64_t res = add(dst,dst,tmp);
+  uint64_t s5 = mul1(tmp,in_a,x);
+  uint64_t res = add(dst,tmp,in_b);
   return (s5 + res);
+}
+
+static inline
+void fadd(uint64_t* dst, const uint64_t* in_a, const uint64_t* in_b) {
+  uint64_t carry = add(dst,in_a,in_b);
+  carry = add1(dst,dst,carry * 38);
+  dst[0] = dst[0] + (carry * 38);
+}
+
+static inline
+void fsub(uint64_t* dst, const uint64_t* in_a, const uint64_t* in_b) {
+  uint64_t carry = sub(dst,in_a,in_b);
+  carry = sub1(dst,dst,carry * 38);
+  dst[0] = dst[0] - (carry * 38);
+}
+
+static inline
+void carry_pass(uint64_t* dst, const uint64_t c_in) {
+  uint64_t carry = add1(dst,dst,c_in * 38);
+  dst[0] = dst[0] + (carry * 38);
+}
+static inline
+void fmul(uint64_t* dst, const uint64_t* in_a, const uint64_t* in_b) {
+  uint64_t tmp[8] = {0};
+  mul(tmp,in_a,in_b);
+  uint64_t carry = mul1_add(dst,tmp+4,38,tmp);
+  carry_pass(dst,carry);
+}
+
+static inline
+void fmul1(uint64_t* dst, const uint64_t* in_a, const uint64_t in_b) {
+  uint64_t carry = mul1(dst,in_a,in_b);
+  carry_pass(dst,carry);
+}
+
+static inline
+void fsqr(uint64_t* dst, const uint64_t* in_a) {
+  uint64_t tmp[8] = {0};
+  sqr(tmp,in_a);
+  uint64_t carry = mul1_add(dst,tmp+4,38,tmp);
+  carry_pass(dst,carry);
 }
 
 static inline
@@ -20,9 +61,39 @@ uint64_t mul2(const uint64_t* dst, const uint64_t* in_a, const uint64_t* in_b) {
   mul(dst+8,in_a+4,in_b+4);
 }
 
+static inline
+void carry_pass2(uint64_t* dst, uint64_t c1, uint64_t c2) {
+  uint64_t carry1 = add1(dst,dst,c1 * 38);
+  uint64_t carry2 = add1(dst+4,dst+4,c2 * 38);
+  dst[0] = dst[0] + (carry1 * 38);
+  dst[0] = dst[0] + (carry2 * 38);
+}
+
+
+static inline
+void fmul2(uint64_t* dst, const uint64_t* in_a, const uint64_t* in_b) {
+  uint64_t tmp[16] = {0};
+  mul2(tmp,in_a,in_b);
+  uint64_t carry1 = mul1_add(dst,tmp+4,38,tmp);
+  uint64_t carry2 = mul1_add(dst+4,tmp+12,38,tmp+8);
+  carry_pass2(dst,carry1,carry2);
+}
 
 static inline
 uint64_t sqr2(const uint64_t* dst, const uint64_t* in_a) {
   sqr(dst,in_a);
   sqr(dst+8,in_a+4);
 }
+
+static inline
+void fsqr2(uint64_t* dst, const uint64_t* in_a) {
+  uint64_t tmp[16] = {0};
+  sqr2(tmp,in_a);
+  uint64_t carry1 = mul1_add(dst,tmp+4,38,tmp);
+  uint64_t carry2 = mul1_add(dst+4,tmp+12,38,tmp+8);
+  carry_pass2(dst,carry1,carry2);
+}
+
+
+
+
