code/experimental/curve25519/Hacl.Impl.Curve25519.Field64.fst
@@ -7,7 +7,8 @@ open Lib.Sequence
 open Lib.IntTypes
 open Lib.Buffer
 open FStar.Mul
-module Core64=Hacl.Impl.Curve25519.Field64.Core
+
+include Hacl.Impl.Curve25519.Field64.Core
 #reset-options "--z3rlimit 20"
 
 
@@ -67,118 +68,6 @@ let copy_felem f1 f2 =
     f1.(size 3) <- f2.(size 3)
 
 
-[@ CInline]
-val fadd: out:felem -> f1:felem  -> f2:felem  -> Stack unit
-          (requires (fun h -> live h f1 /\ live h f2 /\ live h out))
-	  (ensures (fun h0 _ h1 -> modifies (loc out) h0 h1))
-let fadd out f1 f2 =
-  let carry = Core64.add out f1 f2 in
-  let carry = Core64.add1 out out (u64 38 *. carry) in
-  out.(0ul) <- out.(0ul) +. (u64 38 *. carry)
-  
-
-
-[@ CInline]
-val fsub: out:felem ->  f1:felem  -> f2:felem  -> Stack unit
-                   (requires (fun h -> live h f1 /\ live h f2 /\ live h out))
-		   (ensures (fun h0 _ h1 -> modifies (loc out) h0 h1 ))
-[@ CInline]
-let fsub out f1 f2 = 
-  let carry = Core64.sub out f1 f2 in
-  let carry = Core64.sub1 out out (u64 38 *. carry) in
-  out.(0ul) <- out.(0ul) -. (u64 38 *. carry)
-
-
-
-
-[@ CInline]
-val carry_wide: out:felem -> inp:felem_wide -> Stack unit
-                   (requires (fun h -> live h out /\ live h inp))
-		   (ensures (fun h0 _ h1 -> modifies (loc out |+| loc inp) h0 h1))
-[@ CInline]
-let carry_wide out inp =
-  out.(0ul) <- inp.(0ul);
-  out.(1ul) <- inp.(1ul);
-  out.(2ul) <- inp.(2ul);
-  out.(3ul) <- inp.(3ul);
-  let s5 = Core64.mul1_add out (sub inp 4ul 4ul) (u64 38) in
-  let carry = Core64.add1 out out (u64 38 *. s5) in
-  out.(0ul) <- out.(0ul) +. (u64 38 *. carry)
-
-
-[@ CInline]
-val fmul: out:felem -> f1:felem -> f2:felem -> Stack unit
-                   (requires (fun h -> live h out /\ live h f1 /\ live h f2))
-		   (ensures (fun h0 _ h1 -> modifies (loc out) h0 h1))
-[@ CInline]
-let fmul out f1 f2 =
-  push_frame();
-  let tmp_w = create_wide () in
-  Core64.mul tmp_w f1 f2;
-  carry_wide out tmp_w;
-  pop_frame()
-
-[@ CInline]
-val fmul2:
-    out:felem2
-  -> f1:felem2
-  -> f2:felem2
-  -> Stack unit
-  (requires (fun h -> live h out /\ live h f1 /\ live h f2))
-  (ensures (fun h0 _ h1 -> modifies (loc out) h0 h1))
-[@ CInline]
-let fmul2 out f1 f2 =
-  push_frame();
-  let tmp = create 16ul (u64 0) in
-  Core64.mul2 tmp f1 f2;
-  let out1 = sub out 0ul 4ul in
-  let out2 = sub out 4ul 4ul in
-  let tmp1 = sub tmp 0ul 8ul in
-  let tmp2 = sub tmp 8ul 8ul in
-  carry_wide out1 tmp1;
-  carry_wide out2 tmp2;
-  pop_frame()
-
-[@ CInline]
-val fmul1: out:felem -> f1:felem -> f2:uint64 -> Stack unit
-                   (requires (fun h -> live h out /\ live h f1))
-		   (ensures (fun h0 _ h1 -> modifies (loc out) h0 h1))
-[@ CInline]
-let fmul1 out f1 f2 =
-  let s4 = Core64.mul1 out f1 f2 in
-  let carry = Core64.add1 out out (u64 38 *. s4) in
-  out.(0ul) <- out.(0ul) +. carry
-
-[@ CInline]
-val fsqr: out:felem -> f1:felem -> Stack unit
-                   (requires (fun h -> live h out /\ live h f1))
-		   (ensures (fun h0 _ h1 -> modifies (loc out) h0 h1))
-[@ CInline]
-let fsqr out f = 
-  push_frame();
-  let tmp = create_wide () in
-  Core64.sqr tmp f;
-  carry_wide out tmp;
-  pop_frame()
-
-[@ CInline]
-val fsqr2: out:felem2 -> f:felem2 -> Stack unit
-        (requires (fun h -> live h out /\ live h f))
-	(ensures (fun h0 _ h1 -> modifies (loc out) h0 h1))
-[@ CInline]
-let fsqr2 out f = 
-  push_frame();
-  let tmp = create 16ul (u64 0) in
-  let tmp1 = sub tmp 0ul 8ul in
-  let tmp2 = sub tmp 8ul 8ul in
-  let out1 = sub out 0ul 4ul in
-  let out2 = sub out 4ul 4ul in
-  Core64.sqr2 tmp f;
-  carry_wide out1 tmp1;
-  carry_wide out2 tmp2;
-  pop_frame()
- 
-
 inline_for_extraction
 val load_felem: f:felem -> u64s:lbuffer uint64 4ul -> Stack unit
                    (requires (fun h -> live h u64s /\ live h f))
@@ -196,11 +85,11 @@ let store_felem u64s f =
     let f3 = f.(3ul) in
     let top_bit = f3 >>. 63ul in
     f.(3ul) <- f3 &. u64 0x7fffffffffffffff;
-    let carry = Core64.add1 f f (u64 19 *. top_bit) in
+    let carry = add1 f f (u64 19 *. top_bit) in
     let f3 = f.(3ul) in
     let top_bit = f3 >>. 63ul in
     f.(3ul) <- f3 &. u64 0x7fffffffffffffff;
-    let carry = Core64.add1 f f (u64 19 *. top_bit) in
+    let carry = add1 f f (u64 19 *. top_bit) in
     u64s.(0ul) <- f.(0ul);
     u64s.(1ul) <- f.(1ul);
     u64s.(2ul) <- f.(2ul);
