code/experimental/curve25519/Hacl.Impl.Curve25519.Field64.Core.fsti
@@ -13,52 +13,48 @@ let u256 = lbuffer uint64 4ul
 let u512 = lbuffer uint64 8ul
 let u1024 = lbuffer uint64 16ul
 
-[@CInline]
-val add: out:u256 -> f1:u256  -> f2:u256  -> Stack uint64
-          (requires (fun h -> live h f1 /\ live h f2 /\ live h out))
-	  (ensures (fun h0 _ h1 -> modifies (loc out) h0 h1))
-
 [@ CInline]
 val add1: out:u256 -> f1:u256  -> f2:uint64  -> Stack uint64
           (requires (fun h -> live h f1 /\ live h out))
 	  (ensures (fun h0 _ h1 -> modifies (loc out) h0 h1))
 
 [@ CInline]
-val sub: out:u256 -> f1:u256  -> f2:u256  -> Stack uint64
+val fadd: out:u256 -> f1:u256  -> f2:u256  -> Stack unit
           (requires (fun h -> live h f1 /\ live h f2 /\ live h out))
 	  (ensures (fun h0 _ h1 -> modifies (loc out) h0 h1))
 
 [@ CInline]
-val sub1: out:u256 -> f1:u256  -> f2:uint64  -> Stack uint64
-          (requires (fun h -> live h f1 /\ live h out))
-	  (ensures (fun h0 _ h1 -> modifies (loc out) h0 h1))
+val fsub: out:u256 ->  f1:u256  -> f2:u256  -> Stack unit
+                   (requires (fun h -> live h f1 /\ live h f2 /\ live h out))
+		   (ensures (fun h0 _ h1 -> modifies (loc out) h0 h1 ))
 
 [@ CInline]
-val mul1: out:u256 -> f1:u256 -> f2:uint64 -> Stack uint64
-         (requires (fun h -> live h out /\ live h f1))
-         (ensures (fun h0 _ h1 -> modifies (loc out) h0 h1))
+val fmul: out:u256 -> f1:u256 -> f2:u256 -> Stack unit
+                   (requires (fun h -> live h out /\ live h f1 /\ live h f2))
+		   (ensures (fun h0 _ h1 -> modifies (loc out) h0 h1))
+
 
 [@ CInline]
-val mul1_add: out:u256 -> f1:u256 -> f2:uint64 -> Stack uint64
+val fmul2:
+    out:u512
+  -> f1:u512
+  -> f2:u512
+  -> Stack unit
+  (requires (fun h -> live h out /\ live h f1 /\ live h f2))
+  (ensures (fun h0 _ h1 -> modifies (loc out) h0 h1))
+
+
+[@ CInline]
+val fmul1: out:u256 -> f1:u256 -> f2:uint64 -> Stack unit
                    (requires (fun h -> live h out /\ live h f1))
 		   (ensures (fun h0 _ h1 -> modifies (loc out) h0 h1))
 
 [@ CInline]
-val mul: out:u512 -> f1:u256 -> r:u256  -> Stack unit
-         (requires (fun h -> live h out /\ live h f1 /\ live h r))
-         (ensures (fun h0 _ h1 -> modifies (loc out) h0 h1))
+val fsqr: out:u256 -> f1:u256 -> Stack unit
+                   (requires (fun h -> live h out /\ live h f1))
+		   (ensures (fun h0 _ h1 -> modifies (loc out) h0 h1))
 
 [@ CInline]
-val mul2: out:u1024 -> f1:u512 -> f2:u512  -> Stack unit
-         (requires (fun h -> live h out /\ live h f1 /\ live h f2))
-         (ensures (fun h0 _ h1 -> modifies (loc out) h0 h1))
-
-[@ CInline]
-val sqr: out:u512 -> f:u256 -> Stack unit
-         (requires (fun h -> live h out /\ live h f))
-         (ensures (fun h0 _ h1 -> modifies (loc out) h0 h1))
-
-[@ CInline]
-val sqr2: out:u1024 -> f:u512  -> Stack unit
-         (requires (fun h -> live h out /\ live h f))
-         (ensures (fun h0 _ h1 -> modifies (loc out) h0 h1))
+val fsqr2: out:u512 -> f:u512 -> Stack unit
+        (requires (fun h -> live h out /\ live h f))
+	(ensures (fun h0 _ h1 -> modifies (loc out) h0 h1))
